\documentclass{beamer}
\usepackage{amsmath}
\usepackage{xcolor}
\usepackage{cancel}
\title{Sequences}
\subtitle{Intro and Example Problems}

\begin{document}
	\frame {
		\titlepage
	}
	
	\frame {
		\frametitle{Explicit v. Recursive}
		\begin{align*}
			\{2, 4, 6, 8, 10, ... a_{n - 1}, a_n\} \hspace{1in} \{2, 4, 8, 16, 32, ... a_{n - 1}, a_n\}
		\end{align*}
	}
	
	\frame {
		\frametitle{Explicit v. Recursive}
		\begin{align*}
			\{2, 4, 6, 8, 10, ... a_{n - 1}, a_n\} \hspace{1in} \{2, 4, 8, 16, 32, ... a_{n - 1}, a_n\}\\	
			d = 2 \hspace{3.5in} r = 2
		\end{align*}
	}

	\frame {
		\frametitle{Explicit}
		\begin{align*}
			\{2, 4, 6, 8, 10, ... a_{n - 1}, a_n\}\\
			\color{blue}a_n = 2\\
		\end{align*}
	}

	\frame {
		\frametitle{Explicit}
		\begin{align*}
			\{2, 4, 6, 8, 10, ... a_{n - 1}, a_n\}\\
			a_n = 2 + \color{blue} 2n\\
		\end{align*}
	}

	\frame {
		\frametitle{Explicit}
		\begin{align*}
			\{2, 4, 6, 8, 10, ... a_{n - 1}, a_n\}\\
			a_n = 2 + \color{blue} 2n\\
			a_2 = 2 + \color{red} 4
		\end{align*}
	}

	\frame {
		\frametitle{Explicit}
		\begin{align*}
			\{2, 4, 6, 8, 10, ... a_{n - 1}, a_n\}\\
			\color{green}a_n = 2 + 2(n - 1)
		\end{align*}
	}

	\frame {
		\frametitle{Recursive}
		\begin{align*}
			\{2, 4, 6, 8, 10, ... a_{n - 1}, a_n\}\\
			\color{blue} \text{if } n = 1, a_n = 2\\
		\end{align*}
	}

	\frame {
		\frametitle{Recursive}
		\begin{align*}
			\{2, 4, 6, 8, 10, ... a_{n - 1}, a_n\}\\
			\text{if } n = 1, a_n = 2\\
			\color{blue} n > 1\\
		\end{align*}
	}

	\frame {
		\frametitle{Recursive}
		\begin{align*}
			\{2, 4, 6, 8, 10, ... a_{n - 1}, a_n\}\\
			\text{if } n = 1, a_n = 2\\
			\color{blue}\text{if } n > 1\\
			\color{blue}a_n = a_{n - 1}
		\end{align*}
	}

	\frame {
		\frametitle{Recursive}
		\begin{align*}
			\{2, 4, 6, 8, 10, ... a_{n - 1}, a_n\}\\
			\text{if } n = 1, a_n = 2\\
			\color{blue}\text{if } n > 1\\
			\text{let's say we want } a_2\\
			4 = \color{blue} 2 + \text{ something}
		\end{align*}
	}
	
	\frame {
		\frametitle{Recursive}
		\begin{align*}
			\{2, 4, 6, 8, 10, ... a_{n - 1}, a_n\}\\
			\text{if } n = 1, a_n = 2\\
			\text{if } n > 1\\
			a_n = a_{n - 1} \color{blue} + 2\\
		\end{align*}
	}

	\frame {
		\frametitle{Recursive}
		\begin{align*}
			\{2, 4, 6, 8, 10, ... a_{n - 1}, a_n\}\\
			\text{if } n = 1, a_n = 2\\
			\text{if } n > 1\\
			\color{green}a_n = a_{n - 1} + 2\\
		\end{align*}
	}
	
	\frame {
		\frametitle{Recursive}
		Given $a_3 = 1$ and $a_4 = 2$, find the 7th term for the sequence where any given term is the sum of the previous two terms.
	}

	\frame {
		\frametitle{Recursive}
		Given $a_3 = 1$ and $a_4 = 2$, find the 7th term for the sequence where any given term is the sum of the previous two terms.
		\begin{align*}
			\color{blue}a_n = a_{n - 2} + a_{n - 1}
		\end{align*}
	}

	\frame {
		\frametitle{Recursive}
		Given $a_3 = 1$ and $a_4 = 2$, find the 7th term for the sequence where any given term is the sum of the previous two terms.
		\begin{align*}
			a_n = a_{n - 2} + a_{n - 1}\\
			\color{blue}a_7 = a_5 + a_6
		\end{align*}
	}

	\frame {
		\frametitle{Recursive}
		Given $a_3 = 1$ and $a_4 = 2$, find the 7th term for the sequence where any given term is the sum of the previous two terms.
		\begin{align*}
			a_n = a_{n - 2} + a_{n - 1}\\
			a_7 = a_5 + a_6\\
			\color{blue}a_6 = a_5 + a_4\\
		\end{align*}
	}

	\frame {
		\frametitle{Recursive}
		Given $a_3 = 1$ and $a_4 = 2$, find the 7th term for the sequence where any given term is the sum of the previous two terms.
		\begin{align*}
			a_n = a_{n - 2} + a_{n - 1}\\
			a_7 = a_5 + a_6\\
			a_6 = a_5 + a_4\\
			\color{blue}a_5 = a_4  +a_3\\
		\end{align*}
	}

	\frame {
		\frametitle{Recursive}
		Given $a_3 = 1$ and $a_4 = 2$, find the 7th term for the sequence where any given term is the sum of the previous two terms.
		\begin{align*}
			a_n = a_{n - 2} + a_{n - 1}\\
			a_7 = a_5 + a_6\\
			a_6 = a_5 + a_4\\
			\color{blue}a_5 = 3\\
		\end{align*}
	}

	\frame {
		\frametitle{Recursive}
		Given $a_3 = 1$ and $a_4 = 2$, find the 7th term for the sequence where any given term is the sum of the previous two terms.
		\begin{align*}
			a_n = a_{n - 2} + a_{n - 1}\\
			a_7 = a_5 + a_6\\
			\color{blue}a_6 = 3 + 2\\
			a_5 = 3\\
		\end{align*}
	}

	\frame {
		\frametitle{Recursive}
		Given $a_3 = 1$ and $a_4 = 2$, find the 7th term for the sequence where any given term is the sum of the previous two terms.
		\begin{align*}
			a_n = a_{n - 2} + a_{n - 1}\\
			\color{blue}a_7 = 3 + 5\\
			a_6 = 5\\
			a_5 = 3\\
		\end{align*}
	}

	\frame {
		\frametitle{Recursive}
		Given $a_3 = 1$ and $a_4 = 2$, find the 7th term for the sequence where any given term is the sum of the previous two terms.
		\begin{align*}
			\color{green}a_7 = 8
		\end{align*}
	}



	\frame {
		\frametitle{Recursive (Geometric)}
		\begin{align*}
			\{2, 4, 8, 16, 32, ... a_{n - 1}, a_n\}\\
			\text{if } n = 1, a_n = 2\\
			\text{if } n > 1\\
			\color{green}a_n = a_{n - 1} \color{blue}\times \color{green} 2\\
		\end{align*}
	}

	\frame {
		\frametitle{Explicit (Geometric)}
		Write an explicit expression for the following sequence
		\begin{align*}
			\{2, 4, 8, 16, 32, ... a_{n - 1}, a_n\}
		\end{align*}
	}









\end{document}
